Introduced accumulator in MergeSort.merge

MergeSort.v
@@ -1,49 +1,112 @@
 Require Import Arith Div2 List Orders Sorted Permutation Program.
 Require Omega.
 
+Local Hint Constructors StronglySorted.
+
+Lemma Forall_app_iff A (P : A -> Prop) xs ys :
+  Forall P (xs ++ ys) <-> (Forall P xs /\ Forall P ys).
+Proof.
+  split;
+    [ intros; split | intros [ ? ? ] ];
+    apply Forall_forall;
+    intros;
+    repeat match goal with
+    | H : In _ (_ ++ _) |- _ => apply in_app_or in H; destruct H
+    | |- In _ (_ ++ _) => apply in_or_app
+    | HIn : In _ ?xs, HForall : Forall _ ?xs |- _ => eapply Forall_forall in HForall; [| clear HForall ]
+    | HIn : In _ ?ys, HForall : Forall _ (_ ++ ?ys) |- _ => eapply Forall_forall in HForall; [| clear HForall ]
+    | HIn : In _ ?xs, HForall : Forall _ (?xs ++ _) |- _ => eapply Forall_forall in HForall; [| clear HForall ]
+    end; eauto.
+Qed.
+
+Lemma Forall_rev_iff A (P : A -> Prop) xs :
+  Forall P (rev xs) <-> Forall P xs.
+Proof.
+  split;
+    intros HForall;
+    apply Forall_forall;
+    intros ? HIn;
+    apply in_rev in HIn;
+    eapply Forall_forall in HForall;
+    eauto.
+Qed.
+
+Lemma StronglySorted_app A le (xs : list A) ys :
+  StronglySorted le xs ->
+  StronglySorted le ys ->
+  Forall (fun x => Forall (le x) ys) xs ->
+  StronglySorted le (xs ++ ys).
+Proof.
+  induction 1; simpl; intros ? HForall.
+  - eauto.
+  - inversion HForall; subst.
+    constructor; eauto.
+    apply Forall_app_iff.
+    eauto.
+Qed.
+
+Lemma StronglySorted_rev A le (xs : list A) :
+  StronglySorted le xs ->
+  StronglySorted (fun x y => le y x) (rev xs).
+Proof.
+  induction 1 as [| ? ? ? ? HForall ]; simpl.
+  - constructor.
+  - apply StronglySorted_app; eauto.
+    apply Forall_rev_iff.
+    eapply Forall_impl; [| apply HForall ].
+    eauto.
+Qed.
+
 Module MergeSort (Import X : TotalTransitiveLeBool').
   Local Coercion is_true : bool >-> Sortclass.
 
-  Local Hint Constructors Permutation StronglySorted.
+  Local Hint Constructors Permutation.
 
   Definition merge : forall xs, StronglySorted leb xs ->
     forall ys, StronglySorted leb ys ->
-    { zs | StronglySorted leb zs /\ Permutation zs (xs ++ ys) }.
+    forall acc,
+    { ws | exists zs, ws = rev zs ++ acc /\ StronglySorted leb zs /\ Permutation zs (xs ++ ys) }.
   Proof.
     refine (fix merge xs :=
       match xs as xs0 return
         StronglySorted leb xs0 ->
         forall ys, StronglySorted leb ys ->
-        { zs | StronglySorted leb zs
+        forall acc,
+        { ws | exists zs, ws = rev zs ++ acc
+            /\ StronglySorted leb zs
             /\ Permutation zs (xs0 ++ ys) } with
-      | [] => fun _ ys _ => exist _ ys _
+      | [] => fun _ ys _ acc => exist _ (rev_append ys acc) _
       | x :: xs' => fun _ =>
           fix merge' ys :=
             match ys with
-            | [] => fun _ => exist _ (x :: xs') _
-            | y :: ys' => fun _ => 
+            | [] => fun _ acc => exist _ (rev_append xs' (x :: acc)) _
+            | y :: ys' => fun _ acc => 
                 (if x <=? y as b return
                   x <=? y = b ->
-                  { zs | StronglySorted leb zs
+                  { ws | exists zs, ws = rev zs ++ acc
+                      /\ StronglySorted leb zs
                       /\ Permutation zs (x :: xs' ++ y :: ys') }
                 then fun _ =>
-                  let (zs, _) := merge xs' _ (y :: ys') _ in
-                  exist _ (x :: zs) _
+                  let (zs, H) := merge xs' _ (y :: ys') _ (x :: acc) in
+                  exist _ zs _
                 else fun _ =>
-                  let (zs, _) := merge' ys' _ in
-                  exist _ (y :: zs) _) eq_refl
+                  let (zs, _) := merge' ys' _ (y :: acc) in
+                  exist _ zs _) eq_refl
             end
-      end);
-      simpl in *;
-      try clear merge';
-      repeat rewrite app_nil_r in *;
-      repeat match goal with
-      | H : StronglySorted _ (_ :: _) |- _ =>
-          inversion H; clear H; subst
-      | H : _ /\ _ |- _ => destruct H
+      end); try clear merge';
+      try match goal with
+      | H : exists _, _ |- _ => destruct H
       end;
-      repeat split;
-      repeat apply SSorted_cons;
+      [ exists ys | exists (x :: xs') | | | exists (x :: x0) | | exists (y :: x0) ];
+      repeat (simpl in *; match goal with
+      | H : StronglySorted _ (_ :: _) |- _ => inversion H; clear H; subst
+      | H : _ /\ _ |- _ => destruct H
+      | _ => rewrite app_nil_r in *
+      | _ => rewrite rev_append_rev in *
+      | _ => rewrite <- app_assoc
+      | _ => split
+      | _ => apply SSorted_cons
+      end; subst);
       eauto;
       repeat match goal with
       | H : Forall ?P ?l |- _ =>
@@ -53,15 +116,15 @@ Module MergeSort (Import X : TotalTransitiveLeBool').
       | |- Forall _ _ =>
           apply Forall_forall; intros
       end.
-    - apply (Permutation_in _ H0) in H2.
-      apply in_app_iff in H2.
-      destruct H2 as [| HIn]; eauto.
+    - apply (Permutation_in _ H0) in H3.
+      apply in_app_iff in H3.
+      destruct H3 as [| HIn]; eauto.
       inversion HIn; subst; eauto.
       eapply leb_trans; eauto.
     - destruct (leb_total x y); [ congruence |].
-      apply (Permutation_in _ H0) in H2.
-      apply in_app_iff with (l := x :: xs') in H2.
-      destruct H2 as [HIn |]; eauto.
+      apply (Permutation_in _ H0) in H3.
+      apply in_app_iff with (l := x :: xs') in H3.
+      destruct H3 as [HIn |]; eauto.
       inversion HIn; subst; eauto.
       eapply leb_trans; eauto.
     - apply Permutation_cons_app with (l1 := x :: xs').
@@ -79,18 +142,19 @@ Module MergeSort (Import X : TotalTransitiveLeBool').
       | [] => fun _ => exist _ [] _
       | [xs] => fun _ => exist _ [xs] _
       | xs :: xs' :: xss' => fun _ =>
-          let (ys, _) := merge xs _ xs' _ in
+          let (ys, _) := merge xs _ xs' _ [] in
           let (yss, _) := meld xss' _ in
-          exist _ (ys :: yss) _
-      end);
-      simpl in *; clear meld;
-      repeat rewrite app_nil_r in *;
-      repeat match goal with
+          exist _ (rev ys :: yss) _
+      end); clear meld;
+      repeat (simpl in *; match goal with
+      | _ => rewrite app_nil_r in *
+      | _ => rewrite rev_involutive in *
       | H : Forall _ (_ :: _) |- _ =>
           inversion H; clear H; subst
       | H : _ /\ _ |- _ => destruct H
-      end;
-      repeat split; eauto.
+      | H : exists _, _ |- _ => destruct H
+      | _ => split
+      end; subst); eauto.
     rewrite app_assoc.
     apply Permutation_app; eauto.
   Defined.
@@ -172,6 +236,13 @@ Module Nat_as_TTLB <: TotalTransitiveLeBool.
 End Nat_as_TTLB.
 
 Module NatSort := MergeSort Nat_as_TTLB.
+Extract Inductive bool => "bool" ["true" "false"].
+Extract Inductive list => "list" ["[]" "(::)"].
+Extract Constant map => "List.map".
+Extract Constant app => "( @ )".
+Extract Constant rev => "List.rev".
+Extract Constant rev_append => "List.rev_append".
+Extraction (* "mergeSort.ml" *) MergeSort.
 
 (* FUCKIN' HEAVY COMPUTATION *)
 (* Eval compute in NatSort.merge_sort [1; 1; 4; 5; 1; 4]. *)
